Fix bugs in pointer operations
* Equality comparison of NULL and non NULL pointers should be defined
* Pointer comparisons, casts, and truth should only be defined for pointers
  that are alive
* Treat dead pointers as indeterminate values in refinements. The proofs that
  all operations preserve refinement indicate that dead pointers can be indeed
  by replaced by anything without affecting the program's behavior.

addresses.v
@@ -109,9 +109,12 @@ Section address_operations.
     ((addr_byte a1 - addr_byte a2) `div` size_of' Γ a1)%Z.
   Global Arguments addr_minus _ !_ !_ /.
 
-  Definition addr_cast_ok (Γ : env Ti) (σc : type Ti) (a : addr Ti) : Prop :=
-    addr_type_base a >*> σc ∧ addr_byte a `mod` size_of Γ σc = 0.
-  Global Arguments addr_cast_ok _ _ !_ /.
+  Definition addr_cast_ok (Γ : env Ti) (m : M)
+      (σc : type Ti) (a : addr Ti) : Prop :=
+    index_alive m (addr_index a) ∧
+    addr_type_base a >*> σc ∧
+    addr_byte a `mod` size_of Γ σc = 0.
+  Global Arguments addr_cast_ok _ _ _ !_ /.
   Definition addr_cast (σc : type Ti) (a : addr Ti) : addr Ti :=
     let 'Addr o r i τ σ _ := a in Addr o r i τ σ σc.
   Global Arguments addr_cast _ !_ /.
@@ -145,6 +148,7 @@ Section address_operations.
        f !! o = Some (o',r') →
        m1 ⊢ o : τ →
        m2 ⊢ o' : τ' →
+       (index_alive m1 o → index_alive m2 o') →
        ✓{Γ} τ' →
        int_typed (size_of Γ τ') sptrT →
        Γ ⊢ r' : τ' ↣ τ → Γ ⊢ r : τ ↣ σ →
@@ -243,6 +247,11 @@ Section addresses.
     by erewrite <-size_of_weaken
       by eauto using castable_type_valid, ref_typed_type_valid.
   Qed.
+  Lemma addr_dead_weaken Γ m1 m2 a σ :
+    (Γ,m1) ⊢ a : σ → index_alive m2 (addr_index a) →
+    (∀ o τ, m1 ⊢ o : τ → index_alive m2 o → index_alive m1 o) →
+    index_alive m1 (addr_index a).
+  Proof. destruct 1; simpl; eauto. Qed.
   Global Instance addr_strict_dec Γ a : Decision (addr_strict Γ a).
   Proof. unfold addr_strict; apply _. Defined.
   Global Instance addr_is_obj_dec a : Decision (addr_is_obj a).
@@ -485,23 +494,21 @@ Section addresses.
     addr_minus_ok m1 a1 a2 → (∀ o, index_alive m1 o → index_alive m2 o) →
     addr_minus_ok m2 a1 a2.
   Proof. intros [??]; split; eauto. Qed.
-  Lemma addr_minus_weaken Γ1 Γ2 mm1 a1 a2 σ1 σ2 :
+  Lemma addr_minus_weaken Γ1 Γ2 mm1 a1 a2 σ1 :
     ✓ Γ1 → (Γ1,mm1) ⊢ a1 : σ1 →
     Γ1 ⊆ Γ2 → addr_minus Γ1 a1 a2 = addr_minus Γ2 a1 a2.
   Proof.
     intros. unfold addr_minus; simplify_type_equality.
     by erewrite (size_of_weaken Γ1 Γ2) by eauto using addr_typed_type_valid.
   Qed.
-  Lemma addr_cast_ok_uchar Γ a : addr_cast_ok Γ ucharT a.
-  Proof. split. constructor. by rewrite size_of_uchar. Qed.
   Lemma addr_cast_typed Γ m a σ σc :
-    (Γ,m) ⊢ a : σ → addr_cast_ok Γ σc a → (Γ,m) ⊢ addr_cast σc a : σc.
-  Proof. intros [] [??]; constructor; naive_solver. Qed.
-  Lemma addr_cast_ok_weaken Γ1 Γ2 mm1 a σ σc :
-    ✓ Γ1 → (Γ1,mm1) ⊢ a : σ →
-    addr_cast_ok Γ1 σc a → Γ1 ⊆ Γ2 → addr_cast_ok Γ2 σc a.
+    (Γ,m) ⊢ a : σ → addr_cast_ok Γ m σc a → (Γ,m) ⊢ addr_cast σc a : σc.
+  Proof. intros [] (?&?&?); constructor; naive_solver. Qed.
+  Lemma addr_cast_ok_weaken Γ1 Γ2 m1 m2 a σ σc :
+    ✓ Γ1 → (Γ1,m1) ⊢ a : σ → (∀ o, index_alive m1 o → index_alive m2 o) →
+    addr_cast_ok Γ1 m1 σc a → Γ1 ⊆ Γ2 → addr_cast_ok Γ2 m2 σc a.
   Proof.
-    intros ?? [??]; split; auto. by erewrite <-size_of_weaken
+    intros ??? (?&?&?); repeat split; auto. by erewrite <-size_of_weaken
       by eauto using castable_type_valid, addr_typed_type_base_valid.
   Qed.
   Lemma addr_type_cast a σc : type_of (addr_cast σc a) = σc.
@@ -653,7 +660,7 @@ Section addresses.
   Proof. intros ->. by constructor. Qed.
   Lemma addr_refine_eq Γ m a1 a2 σ : a1 ⊑{Γ@m} a2 : σ → a1 = a2.
   Proof.
-    destruct 1 as [o o' r' r r'' i i'' τ τ' σ σc ??????????? []];
+    destruct 1 as [o o' r' r r'' i i'' τ τ' σ σc ???????????? []];
       simplify_type_equality'.
     * by rewrite Nat.mul_0_r, Nat.add_0_r.
     * by rewrite (right_id_L [] (++)).
@@ -672,7 +679,7 @@ Section addresses.
   Lemma addr_refine_typed_r Γ f m1 m2 a1 a2 σ :
     ✓ Γ → a1 ⊑{Γ,f@m1↦m2} a2 : σ → (Γ,m2) ⊢ a2 : σ.
   Proof.
-    destruct 2 as [o o' r r' r'' i i'' τ τ' σ σc ??????????? Hr''].
+    destruct 2 as [o o' r r' r'' i i'' τ τ' σ σc ???????????? Hr''].
     assert (ref_offset (freeze true <$> r') < ref_size (freeze true <$> r')).
     { intros. eapply ref_typed_size, ref_typed_freeze; eauto. }
     constructor; auto.
@@ -701,7 +708,7 @@ Section addresses.
     a1 ⊑{Γ,f@m1↦m2} a2 : σ → frozen a1 ↔ frozen a2.
   Proof.
     unfold frozen.
-    destruct 1 as [o o' r' r r'' i i'' τ τ' σ σc ??????????? []]; csimpl.
+    destruct 1 as [o o' r' r r'' i i'' τ τ' σ σc ???????????? []]; csimpl.
     * by rewrite ref_set_offset_freeze, ref_freeze_freeze.
     * rewrite fmap_app, ref_freeze_freeze.
       by split; intro; simplify_list_equality'; repeat f_equal.
@@ -717,8 +724,8 @@ Section addresses.
     a1 ⊑{Γ,f@m1↦m2} a2 : σ → a2 ⊑{Γ,g@m2↦m3} a3 : σ →
     a1 ⊑{Γ,f ◎ g@m1↦m3} a3 : σ.
   Proof.
-    destruct 1 as [o o2 r r2 r3 i i3 τ τ2 σ σc ??????????? Hr3];
-      inversion 1 as [? o4 ? r4 r5 ? i5 ? τ3 ????????????? Hr5]; subst.
+    destruct 1 as [o o2 r r2 r3 i i3 τ τ2 σ σc ???????????? Hr3];
+      inversion 1 as [? o4 ? r4 r5 ? i5 ? τ3 ?????????????? Hr5]; subst.
     exists (r2 ++ r4); auto.
     { by rewrite lookup_mem_inj_compose; simplify_option_equality. }
     { rewrite ref_typed_app; eauto. }
@@ -731,9 +738,10 @@ Section addresses.
   Lemma addr_refine_weaken Γ Γ' f f' m1 m2 m1' m2' a1 a2 σ :
     ✓ Γ → a1 ⊑{Γ,f@m1↦m2} a2 : σ → Γ ⊆ Γ' → f ⊆ f' →
     (∀ o τ, m1 ⊢ o : τ → m1' ⊢ o : τ) → (∀ o τ, m2 ⊢ o : τ → m2' ⊢ o : τ) →
+    (∀ o1 o2 r, f !! o1 = Some (o2,r) → index_alive m1' o1 → index_alive m2' o2) →
     a1 ⊑{Γ',f'@m1'↦m2'} a2 : σ.
   Proof.
-    destruct 2 as [o o2 r r2 r3 i i3 τ τ2 σ σc ????????? Hsz];
+    destruct 2 as [o o2 r r2 r3 i i3 τ τ2 σ σc ?????????? Hsz];
       intros; econstructor; eauto using type_valid_weaken, ref_typed_weaken.
     * by erewrite <-size_of_weaken by eauto.
     * by erewrite <-size_of_weaken by eauto using ref_typed_type_valid.
@@ -744,14 +752,14 @@ Section addresses.
   Lemma addr_refine_unique Γ f m1 m2 a1 a2 a3 σ2 σ3 :
     a1 ⊑{Γ,f@m1↦m2} a2 : σ2 → a1 ⊑{Γ,f@m1↦m2} a3 : σ3 → a2 = a3.
   Proof.
-    destruct 1 as [?????????????????????? []];
-      inversion 1 as [?????????????????????? Hr2]; inversion Hr2;
+    destruct 1 as [??????????????????????? []];
+      inversion 1 as [??????????????????????? Hr2]; inversion Hr2;
       simplify_type_equality'; naive_solver.
   Qed.
   Lemma addr_freeze_refine Γ f m1 m2 a1 a2 σ :
     a1 ⊑{Γ,f@m1↦m2} a2 : σ → freeze true a1 ⊑{Γ,f@m1↦m2} freeze true a2 : σ.
   Proof.
-    intros Ha. destruct Ha as [o o' r r' r'' i i'' τ τ' σ σc ??????????? Hr''];
+    intros Ha. destruct Ha as [o o' r r' r'' i i'' τ τ' σ σc ???????????? Hr''];
       csimpl; econstructor; eauto;
       rewrite ?ref_typed_freeze, ?ref_offset_freeze, ?ref_size_freeze; auto.
     destruct Hr'' as [|r'' i'']; csimpl.
@@ -765,7 +773,7 @@ Section addresses.
     ∃ r, f !! addr_index a1 = Some (addr_index a2, r)
       ∧ addr_ref Γ a2 = addr_ref Γ a1 ++ freeze true <$> r.
   Proof.
-    intros [?? r r' r'' i i'' τ τ' σ' ???????????? Hr''] ?; simplify_equality'.
+    intros [?? r r' r'' i i'' τ τ' σ' ????????????? Hr''] ?; simplify_equality'.
     exists r'; split; auto. destruct Hr''; simplify_equality'; auto.
     rewrite Nat.mul_comm, Nat.div_add, Nat.div_small, Nat.add_0_l by lia.
     by rewrite ref_set_offset_set_offset, ref_set_offset_offset.
@@ -774,7 +782,7 @@ Section addresses.
     a1 ⊑{Γ,f@m1↦m2} a2 : σ → addr_strict Γ a1 →
     addr_ref_byte Γ a1 = addr_ref_byte Γ a2.
   Proof.
-    intros [?? r r' r'' i i'' τ τ' σ' ???????????? Hr''] ?;
+    intros [?? r r' r'' i i'' τ τ' σ' ????????????? Hr''] ?;
       simplify_equality'; destruct Hr''; simplify_equality'; auto.
     by rewrite Nat.mul_comm, Nat.mod_add by lia.
   Qed.
@@ -827,7 +835,7 @@ Section addresses.
       ≤ size_of Γ (addr_type_base a2) * ref_size (addr_ref_base a2)
     ∧ addr_byte a2 = i + addr_byte a1.
   Proof.
-    destruct 1 as [o o' r r' r'' i i'' τ τ' σ' σc ??????????? Hr''].
+    destruct 1 as [o o' r r' r'' i i'' τ τ' σ' σc ???????????? Hr''].
     destruct Hr'' as [|r'' i'']; simplify_type_equality'; [|by exists 0].
     rewrite ref_size_set_offset.
     exists (size_of Γ σ' * ref_offset (freeze true <$> r')). split; [|lia].
@@ -840,20 +848,23 @@ Section addresses.
     intros. destruct (addr_byte_refine_help Γ f m1 m2 a1 a2 σ) as (i&?&?); auto.
     unfold addr_strict in *; lia.
   Qed.
+  Lemma addr_alive_refine Γ f m1 m2 a1 a2 σ :
+    index_alive m1 (addr_index a1) → a1 ⊑{Γ,f@m1↦m2} a2 : σ →
+    index_alive m2 (addr_index a2).
+  Proof. destruct 2; auto. Qed.
   Lemma addr_plus_ok_refine Γ f m1 m2 a1 a2 σ j :
-    ✓ Γ → m1 ⊑{Γ,f} m2 → a1 ⊑{Γ,f@m1↦m2} a2 : σ →
-    addr_plus_ok Γ m1 j a1 → addr_plus_ok Γ m2 j a2.
+    a1 ⊑{Γ,f@m1↦m2} a2 : σ → addr_plus_ok Γ m1 j a1 → addr_plus_ok Γ m2 j a2.
   Proof.
-    unfold addr_plus_ok. intros ?? Ha (?&?&?).
+    unfold addr_plus_ok. intros Ha (?&?&?).
     destruct (addr_byte_refine_help Γ f m1 m2 a1 a2 σ) as (i&?&?); auto.
-    destruct Ha; simplify_equality'. split. eauto using mem_refine_alive. lia.
+    destruct Ha; simplify_equality'. split; eauto with lia.
   Qed.
   Lemma addr_plus_refine Γ f m1 m2 a1 a2 σ j :
-    ✓ Γ → m1 ⊑{Γ,f} m2 → addr_plus_ok Γ m1 j a1 →
+    ✓ Γ → addr_plus_ok Γ m1 j a1 →
     a1 ⊑{Γ,f@m1↦m2} a2 : σ → addr_plus Γ j a1 ⊑{Γ,f@m1↦m2} addr_plus Γ j a2 : σ.
   Proof.
-    intros ?? Ha' Ha. destruct Ha' as (_&?&?), Ha as
-      [o o' r r' r'' i i'' τ τ' σ σc ??????????? Hr'']; simplify_equality'.
+    intros ? Ha' Ha. destruct Ha' as (_&?&?), Ha as
+      [o o' r r' r'' i i'' τ τ' σ σc ???????????? Hr'']; simplify_equality'.
     econstructor; eauto.
     { apply Nat2Z.inj_le. by rewrite Nat2Z.inj_mul, Z2Nat.id by done. }
     { apply Nat2Z.inj. rewrite Z2Nat_inj_mod, Z2Nat.id by done.
@@ -869,44 +880,44 @@ Section addresses.
       by auto using Z.mul_nonneg_nonneg with lia.
   Qed.
   Lemma addr_minus_ok_refine Γ f m1 m2 a1 a2 a3 a4 σ :
-    ✓ Γ → m1 ⊑{Γ,f} m2 → a1 ⊑{Γ,f@m1↦m2} a2 : σ → a3 ⊑{Γ,f@m1↦m2} a4 : σ →
+    a1 ⊑{Γ,f@m1↦m2} a2 : σ → a3 ⊑{Γ,f@m1↦m2} a4 : σ →
     addr_minus_ok m1 a1 a3 → addr_minus_ok m2 a2 a4.
   Proof.
-    destruct 3 as [?????????????????????? []],
-      1 as [?????????????????????? []]; intros (?&?&Hr);
-      simplify_equality'; eauto using mem_refine_alive.
-    rewrite !fmap_app, !ref_freeze_freeze by eauto.
-    split. eauto using mem_refine_alive. intuition congruence.
+    destruct 1 as [??????????????????????? []], 1 as
+      [??????????????????????? []]; intros (?&?&Hr); simplify_equality'; eauto.
+    rewrite !fmap_app, !ref_freeze_freeze by eauto. intuition congruence.
   Qed.
   Lemma addr_minus_refine Γ f m1 m2 a1 a2 a3 a4 σ :
-    ✓ Γ → addr_minus_ok m1 a1 a3 →
-    a1 ⊑{Γ,f@m1↦m2} a2 : σ → a3 ⊑{Γ,f@m1↦m2} a4 : σ →
-    addr_minus Γ a1 a3 = addr_minus Γ a2 a4.
+    addr_minus_ok m1 a1 a3 → a1 ⊑{Γ,f@m1↦m2} a2 : σ →
+    a3 ⊑{Γ,f@m1↦m2} a4 : σ → addr_minus Γ a1 a3 = addr_minus Γ a2 a4.
   Proof.
-    intros ? (?&?&?).
-    destruct 1 as [o1 o2 r1 r2 r3 i1 i3 τ1 τ2 σ1 σc ??????????? Hr3],
-      1 as [o4 o5 r4 r5 r6 i4 i6 τ4 τ5 σ3 σc4 ??????????? Hr6].
+    intros (?&?&?).
+    destruct 1 as [o1 o2 r1 r2 r3 i1 i3 τ1 τ2 σ1 σc ???????????? Hr3],
+      1 as [o4 o5 r4 r5 r6 i4 i6 τ4 τ5 σ3 σc4 ???????????? Hr6].
     destruct Hr3, Hr6; simplify_type_equality'; f_equal; lia.
   Qed.
   Lemma addr_cast_ok_refine Γ f m1 m2 a1 a2 σ σc :
-    a1 ⊑{Γ,f@m1↦m2} a2 : σ → addr_cast_ok Γ σc a1 → addr_cast_ok Γ σc a2.
+    ✓ Γ → a1 ⊑{Γ,f@m1↦m2} a2 : σ →
+    addr_cast_ok Γ m1 σc a1 → addr_cast_ok Γ m2 σc a2.
   Proof.
-    destruct 1 as [o o' r r' r'' i i'' τ τ' σ σc' ??????????? []];
-      intros (?&?); simplify_equality'; split_ands; auto.
+    destruct 2 as [o o' r r' r'' i i'' τ τ' σ σc' ???????????? []];
+      intros (?&?&?); simplify_equality'; split_ands; eauto.
     destruct (castable_divide Γ σ σc) as [z ->]; auto.
     rewrite ref_offset_freeze.
     destruct (decide (size_of Γ σc = 0)) as [->|?]; [done|].
     by rewrite !(Nat.mul_comm (_ * size_of _ _)), Nat.mul_assoc, Nat.mod_add.
   Qed.
   Lemma addr_cast_refine Γ f m1 m2 a1 a2 σ σc :
-    addr_cast_ok Γ σc a1 → a1 ⊑{Γ,f@m1↦m2} a2 : σ →
+    addr_cast_ok Γ m1 σc a1 → a1 ⊑{Γ,f@m1↦m2} a2 : σ →
     addr_cast σc a1 ⊑{Γ,f@m1↦m2} addr_cast σc a2 : σc.
-  Proof. intros [??]. destruct 1; simplify_equality'; econstructor; eauto. Qed.
+  Proof.
+    intros (?&?&?). destruct 1; simplify_equality'; econstructor; eauto.
+  Qed.
   Lemma addr_elt_refine Γ f m1 m2 a1 a2 σ n :
     ✓ Γ → addr_strict Γ a1 → a1 ⊑{Γ,f@m1↦m2} a2 : σ.[n] →
     addr_elt Γ a1 ⊑{Γ,f@m1↦m2} addr_elt Γ a2 : σ.
   Proof.
-    inversion 3 as [o o' r r' r'' i i'' τ τ' ???????????? Hc Hr''];
+    inversion 3 as [o o' r r' r'' i i'' τ τ' ????????????? Hc Hr''];
       inversion Hc; clear Hc; simplify_equality'.
     assert (✓{Γ} σ ∧ n ≠ 0) as [??]
       by eauto using TArray_valid_inv, ref_typed_type_valid.
@@ -928,7 +939,7 @@ Section addresses.
     a1 ⊑{Γ,f@m1↦m2} a2 : compoundT{c} s → Γ !! s = Some σs → σs !! j = Some σ →
     addr_field Γ j a1 ⊑{Γ,f@m1↦m2} addr_field Γ j a2 : σ.
   Proof.
-    inversion 3 as [o o' r r' r'' i i'' τ τ' ???????????? Hc Hr''];
+    inversion 3 as [o o' r r' r'' i i'' τ τ' ????????????? Hc Hr''];
       inversion Hc; clear Hc; intros; simplify_option_equality.
     econstructor; eauto using env_valid_lookup_lookup.
     * apply ref_typed_cons; eexists (compoundT{c} s); split.
